\documentclass{article}
\usepackage{epsfig}
\pagestyle{empty}
\begin{document}
\[ \log({\mathrm{likelihood}}) = \sum_{i = 1}^n \frac{\left(g\left(m\right)_i - d_i\right)^2}{2 \sigma_i^2} \]
\pagebreak

\[ \Pr(d|m) = \frac{1}{\prod_{i=1}^n \sqrt{2 \pi \cdot \sigma_i^2}} \exp{\left( \sum_{i = 1}^n \frac{-\left(g\left(m\right)_i - d_i\right)^2}{2\sigma_i^2}\right)} \]
\pagebreak

$g(m)_i$
\pagebreak

$d_i$
\pagebreak

$\sigma_i$
\pagebreak

$\sigma$
\pagebreak

\[ \Pr() = \frac{1}{(2 \pi)^{n/2} |C_e|} \exp{-\frac{1}{2}(g(m) - d)^T C_e^{-1} (g(m) - d)} \]
\pagebreak

$ C_e $
\pagebreak

$\frac{1}{2}(g(m) - d)^T C_e^{-1} (g(m) - d)$
\pagebreak

$d$
\pagebreak

$m$
\pagebreak

$\lambda$
\pagebreak

\[ \Pr(d|m) = \frac{1}{\prod_{i=1}^n \sqrt{2 \pi \cdot (\lambda \cdot \sigma_i)^2}} \exp{\left( \sum_{i = 1}^n \frac{-\left(g\left(m\right)_i - d_i\right)^2}{2(\lambda \cdot \sigma_i)^2}\right)} \]
\pagebreak

\end{document}
